theories/paperintro.v
@@ -1,0 +1,28 @@
+From Equations Require Import Equations.
+
+Inductive ty : Type :=
+| arrow : ty -> ty -> ty
+| base : ty.
+
+Derive NoConfusion for ty.
+
+Definition ctx := list ty.
+
+Inductive Deriv : ctx -> ty -> Type :=
+| var : forall ctx ty, List.In ty ctx -> Deriv ctx ty
+| lambda : forall {ctx A B}, Deriv (cons A ctx) B -> Deriv ctx (arrow A B)
+| application : forall {ctx A B}, Deriv ctx (arrow A B) -> Deriv ctx A -> Deriv ctx B
+| tt : forall ctx, Deriv ctx base.
+
+Axiom substitute : forall {ctx A B}, Deriv ctx A -> Deriv (cons A ctx) B -> Deriv ctx B.
+
+Equations betaReduce : forall {ctx ty}, Deriv ctx ty -> Deriv ctx ty :=
+betaReduce (application (lambda t1) t2) := substitute t2 t1;
+betaReduce t := t.
+
+Search (_ -> list _ -> Prop).
+
+Theorem test (H :  2 + 2 + 2 + 2 + 2 + 2 + 2 + 2 + 2 = 2 + 2 + 2
+             + 2 + 2 + 2 + 2 + 2 + 2 + 2 + 2 + 2 + 2 + 2 + 2 + 2 + 2 + 2 + 2 + 2
+             + 2 + 2 + 2 + 2 + 2 ) : 1 = 1.
+Proof.
